Checkpoint before generalizing push property

StrictPositivity.v
@@ -24,13 +24,17 @@ Require Import Termination.ErasedTermLemmas.
 Require Import Termination.ReducibilityCandidate.
 Require Import Termination.ReducibilityDefinition.
 Require Import Termination.ReducibilityLemmas.
-Require Import Termination.ReducibilityUnused.
-Require Import Termination.ReducibilityMeasure.
-Require Import Termination.ReducibilityRenaming.
-Require Import Termination.ReducibilitySubst.
 Require Import Termination.RedTactics.
+Require Import Termination.ReducibilityMeasure.
+Require Import Termination.ReducibilitySubst.
+Require Import Termination.ReducibilityRenaming.
+Require Import Termination.ReducibilityUnused.
 Require Import Termination.RedTactics2.
 
+Require Import Termination.IdRelation.
+Require Import Termination.EqualWithRelation.
+
+Require Import Termination.EquivalentWithRelation.
 Require Import Termination.AssocList.
 Require Import Termination.Sets.
 Require Import Termination.Freshness.
@@ -44,81 +48,123 @@ Opaque makeFresh.
 Opaque Nat.eq_dec.
 Opaque reducible_values.
 
-Fixpoint no_type_lvar (t: tree) (k: nat) :=
-  match t with
-  | fvar _ type_var => True
-  | lvar i type_var => i <> k
+Definition no_type_fvar T vars :=
+  forall X, X ∈ pfv T type_var -> X ∈ vars -> False.
 
-  | T_unit => True
-  | T_bool => True
-  | T_nat => True
-  | T_prod T1 T2 => no_type_lvar T1 k /\ no_type_lvar T2 k
-  | T_arrow T1 T2 => no_type_lvar T1 k /\ no_type_lvar T2 k
-  | T_sum T1 T2 => no_type_lvar T1 k /\ no_type_lvar T2 k
-  | T_refine T p => no_type_lvar T k
-  | T_let t A B => no_type_lvar A k /\ no_type_lvar B k
-  | T_singleton t => True
-  | T_intersection T1 T2 => no_type_lvar T1 k /\ no_type_lvar T2 k
-  | T_union T1 T2 => no_type_lvar T1 k /\ no_type_lvar T2 k
-  | T_top => True
-  | T_bot => True
-  | T_equal t1 t2 => True
-  | T_forall T1 T2 => no_type_lvar T1 k /\ no_type_lvar T2 k
-  | T_exists T1 T2 => no_type_lvar T1 k /\ no_type_lvar T2 k
-  | T_abs T => no_type_lvar T (S k)
-  | T_rec n T0 Ts => no_type_lvar T0 k /\ no_type_lvar Ts (S k)
+Equations strictly_positive (T: tree) (vars: list nat): Prop
+    by wf (size T) lt :=
+  strictly_positive (fvar _ type_var) _ := True;
+  strictly_positive (lvar _ _) _ := True;
 
-  | _ => False
-  end.
+  strictly_positive T_unit _ := True;
+  strictly_positive T_bool _ := True;
+  strictly_positive T_nat _ := True;
+  strictly_positive T_top _ := True;
+  strictly_positive T_bot _ := True;
+  strictly_positive (T_equal _ _) _ := True;
 
-Fixpoint strictly_positive (t: tree) (k: nat) :=
-  match t with
-  | fvar _ type_var => True
-  | lvar i type_var => True
+  strictly_positive (T_prod T1 T2) vars := strictly_positive T1 vars /\ strictly_positive T2 vars;
+  strictly_positive (T_arrow T1 T2) vars := no_type_fvar T1 vars /\ strictly_positive T2 vars;
+  strictly_positive (T_forall T1 T2) vars := no_type_fvar T1 vars /\ strictly_positive T2 vars;
+  strictly_positive (T_sum T1 T2) vars := strictly_positive T1 vars /\ strictly_positive T2 vars;
+  strictly_positive (T_refine T p) vars := strictly_positive T vars;
+  strictly_positive (T_let t T1 T2) vars :=
+    strictly_positive T1 vars /\ strictly_positive T2 vars;
+  strictly_positive (T_singleton _) _ := True;
+  strictly_positive (T_intersection T1 T2) _ :=
+    strictly_positive T1 vars /\ strictly_positive T2 vars;
 
-  | T_unit => True
-  | T_bool => True
-  | T_nat => True
-  | T_prod T1 T2 => strictly_positive T1 k /\ strictly_positive T2 k
-  | T_arrow T1 T2 => no_type_lvar T1 k /\ strictly_positive T2 k
-  | T_sum T1 T2 => strictly_positive T1 k /\ strictly_positive T2 k
-  | T_refine T p => strictly_positive T k
-  | T_let t A B => strictly_positive A k /\ strictly_positive B k
-  | T_singleton t => True
-  | T_intersection T1 T2 => strictly_positive T1 k /\ strictly_positive T2 k
-  | T_union T1 T2 => no_type_lvar T1 k /\ no_type_lvar T2 k (* !! TODO: This could be relaxed by letting one hole in either T1 or T2 *)
-  | T_top => True
-  | T_bot => True
-  | T_equal t1 t2 => True
-  | T_forall T1 T2 => no_type_lvar T1 k /\ strictly_positive T2 k
-  | T_exists T1 T2 => no_type_lvar T1 k /\ no_type_lvar T2 k (* !! We cannot push foralls down exists *)
-  | T_abs T => strictly_positive T (S k)
-  | T_rec n T0 Ts => strictly_positive T0 k /\ strictly_positive Ts (S k) /\ (
-                    (* if (S k) appears in Ts, then the recursive type variable of Ts must be positive*)
-                      no_type_lvar Ts (S k) \/ strictly_positive Ts 0
-                    )
+  (* could be relaxed *)
+  strictly_positive (T_union T1 T2) vars :=
+    no_type_fvar T1 vars /\ no_type_fvar T2 vars;
+  strictly_positive (T_exists T1 T2) vars := no_type_fvar T1 vars /\ no_type_fvar T2 vars;
 
-  | _ => False
-  end.
+  strictly_positive (T_abs T) vars := strictly_positive T vars;
+  strictly_positive (T_rec n T0 Ts) vars :=
+    strictly_positive T0 vars /\ strictly_positive Ts vars /\ (
+      (no_type_fvar T0 vars /\ no_type_fvar Ts vars) \/
+      exists X,
+        ~(X ∈ pfv Ts type_var) /\
+        strictly_positive (topen 0 Ts (fvar X type_var)) (X :: nil)
+    );
 
-Lemma no_type_lvar_open:
-  forall T k1 k2 rep,
-    twf rep 0 ->
-    no_type_lvar T k1 ->
-    no_type_lvar (open k2 T rep) k1.
+  strictly_positive _ vars := False.
+
+
+Solve All Obligations with (repeat step || autorewrite with bsize in *; try omega; eauto with omega).
+Fail Next Obligation.
+
+Ltac simp_spos :=
+  rewrite strictly_positive_equation_1 in * ||
+  rewrite strictly_positive_equation_2 in * ||
+  rewrite strictly_positive_equation_3 in * ||
+  rewrite strictly_positive_equation_4 in * ||
+  rewrite strictly_positive_equation_5 in * ||
+  rewrite strictly_positive_equation_6 in * ||
+  rewrite strictly_positive_equation_7 in * ||
+  rewrite strictly_positive_equation_8 in * ||
+  rewrite strictly_positive_equation_9 in * ||
+  rewrite strictly_positive_equation_10 in * ||
+  rewrite strictly_positive_equation_11 in * ||
+  rewrite strictly_positive_equation_12 in * ||
+  rewrite strictly_positive_equation_13 in * ||
+  rewrite strictly_positive_equation_14 in * ||
+  rewrite strictly_positive_equation_15 in * ||
+  rewrite strictly_positive_equation_16 in * ||
+  rewrite strictly_positive_equation_17 in * ||
+  rewrite strictly_positive_equation_18 in * ||
+  rewrite strictly_positive_equation_19 in * ||
+  rewrite strictly_positive_equation_20 in * ||
+  rewrite strictly_positive_equation_21 in * ||
+  rewrite strictly_positive_equation_22 in * ||
+  rewrite strictly_positive_equation_23 in * ||
+  rewrite strictly_positive_equation_24 in * ||
+  rewrite strictly_positive_equation_25 in * ||
+  rewrite strictly_positive_equation_26 in * ||
+  rewrite strictly_positive_equation_27 in * ||
+  rewrite strictly_positive_equation_28 in * ||
+  rewrite strictly_positive_equation_29 in * ||
+  rewrite strictly_positive_equation_30 in * ||
+  rewrite strictly_positive_equation_31 in * ||
+  rewrite strictly_positive_equation_32 in * ||
+  rewrite strictly_positive_equation_33 in * ||
+  rewrite strictly_positive_equation_34 in * ||
+  rewrite strictly_positive_equation_35 in * ||
+  rewrite strictly_positive_equation_36 in * ||
+  rewrite strictly_positive_equation_37 in * ||
+  rewrite strictly_positive_equation_38 in * ||
+  rewrite strictly_positive_equation_39 in * ||
+  rewrite strictly_positive_equation_40 in * ||
+  rewrite strictly_positive_equation_41 in * ||
+  rewrite strictly_positive_equation_42 in * ||
+  rewrite strictly_positive_equation_43 in * ||
+  rewrite strictly_positive_equation_44 in * ||
+  rewrite strictly_positive_equation_45 in * ||
+  rewrite strictly_positive_equation_46 in * ||
+  rewrite strictly_positive_equation_47 in * ||
+  rewrite strictly_positive_equation_48 in * ||
+  rewrite strictly_positive_equation_49 in * ||
+  rewrite strictly_positive_equation_50 in *.
+
+Opaque strictly_positive.
+
+Lemma is_erased_term_no_type_fvar:
+  forall t vars,
+    is_erased_term t ->
+    no_type_fvar t vars.
 Proof.
-  induction T; steps; eauto using twf_open with btwf omega.
+  unfold no_type_fvar; repeat step || rewrite is_erased_term_tfv in *.
 Qed.
 
-Lemma strictly_positive_open:
-  forall T k1 k2 rep,
-    twf rep 0 ->
-    strictly_positive T k1 ->
-    strictly_positive (open k2 T rep) k1.
+Lemma no_type_fvar_open:
+  forall T vars rep k,
+    is_erased_term rep ->
+    no_type_fvar T vars ->
+    no_type_fvar (open k T rep) vars.
 Proof.
-  induction T; steps;
-    eauto using twf_open with btwf omega;
-    eauto using no_type_lvar_open.
+  unfold no_type_fvar;
+    repeat step || t_fv_open || t_listutils ||
+           rewrite is_erased_term_tfv in * by steps; eauto.
 Qed.
 
 Definition non_empty theta A := exists v, reducible_values theta v A.
@@ -138,49 +184,6 @@ Ltac t_instantiate_non_empty :=
     pose proof (instantiate_non_empty _ _ _ H1 H2)
   end.
 
-Ltac apply_induction H :=
-  match goal with
-  | |- reducible_values _ _ (topen 0 ?T _) => apply H with (size T, index T)
-  end.
-
-(*
-Lemma twf_positive:
-  forall T k,
-    is_erased_type T ->
-    twf T k ->
-    strictly_positive T k.
-Proof.
-  induction T; steps; try omega.
-Qed.
-*)
-
-(*
-Lemma strict_positive_monotone:
-  forall T k1 k2,
-    strictly_positive T k1 ->
-    k1 <= k2 ->
-    strictly_positive T k2.
-Proof.
-  induction T;
-    repeat step;
-    eauto with btwf omega.
-Qed.
-*)
-
-(*
-Lemma strictly_positive_swap:
-  forall T i rep,
-    twf rep 0 ->
-    is_erased_type T ->
-    strictly_positive rep 0 ->
-    strictly_positive T (S i) ->
-    strictly_positive (topen (S i) (swap_type_holes T i (S i)) rep) i.
-Proof.
-  induction T; repeat step || apply twf_swap;
-    eauto using strict_positive_monotone with omega.
-Qed.
-*)
-
 Lemma non_empty_extend:
   forall theta A x RC,
     non_empty theta A ->
@@ -192,295 +195,637 @@ Proof.
   unfold non_empty; repeat step || exists v || apply reducible_unused2.
 Qed.
 
-Lemma twf_no_type_lvar:
-  forall T k,
-    is_erased_type T ->
-    twf T k ->
-    no_type_lvar T k.
+Definition push_one (a: tree) (l: list (nat * (tree -> tree -> Prop))): interpretation :=
+  mapValues (fun rc => rc a) l.
+
+Definition push_all (P: tree -> Prop) (l: list (nat * (tree -> tree -> Prop))): interpretation :=
+  mapValues (fun (rc: tree -> tree -> Prop) (v: tree) => (forall a, P a -> rc a v)) l.
+
+Fixpoint valid_pre_interpretation (P: tree -> Prop) (theta: list (nat * (tree -> tree -> Prop))) : Prop :=
+  match theta with
+  | nil => True
+  | (_, RC) :: theta' => valid_pre_interpretation P theta' /\ forall a, P a -> reducibility_candidate (RC a)
+  end.
+
+Lemma valid_interpretation_one:
+  forall a (P: tree -> Prop) theta,
+    P a ->
+    valid_pre_interpretation P theta ->
+    valid_interpretation (push_one a theta).
 Proof.
-  induction T; steps; try omega.
+  induction theta; steps.
 Qed.
 
-Lemma twf_positive:
-  forall T k,
-    is_erased_type T ->
-    twf T k ->
-    strictly_positive T k.
+Definition sat { X } (P: X -> Prop) := exists x, P x.
+
+Lemma valid_interpretation_all:
+  forall (P: tree -> Prop) theta,
+    sat P ->
+    valid_pre_interpretation P theta ->
+    valid_interpretation (push_all P theta).
 Proof.
-  induction T; steps; try omega;
-    eauto using twf_no_type_lvar.
+  unfold sat; induction theta;
+    repeat step || unfold reducibility_candidate in * || instantiate_any.
 Qed.
 
-Lemma twf_positive2:
-  forall T k,
-    is_erased_type T ->
-    twf T 0 ->
-    strictly_positive T k.
+Lemma valid_interpretation_append:
+  forall theta1 theta2,
+    valid_interpretation theta1 ->
+    valid_interpretation theta2 ->
+    valid_interpretation (theta1 ++ theta2).
 Proof.
-  eauto using twf_positive with btwf omega.
+  induction theta1; steps.
 Qed.
 
-Lemma no_type_lvar_in_topen:
-  forall T i j R,
-    is_erased_type T ->
-    is_erased_type R ->
-    twf R 0 ->
-    no_type_lvar T i ->
-    no_type_lvar (topen j T R) i.
+Lemma valid_interpretation_all2:
+  forall theta theta' A,
+    non_empty theta A ->
+    valid_interpretation theta ->
+    valid_pre_interpretation (fun a => reducible_values theta a A) theta' ->
+    valid_interpretation (push_all (fun a => reducible_values theta a A) theta' ++ theta).
 Proof.
-  induction T; repeat step || apply twf_no_type_lvar;
-    eauto using twf_positive2; eauto with btwf omega.
+  repeat step || apply valid_interpretation_append || apply valid_interpretation_all || unfold sat.
+Qed.
+
+Hint Resolve valid_interpretation_cons: b_valid_interp.
+Hint Resolve valid_interpretation_one: b_valid_interp.
+Hint Resolve valid_interpretation_all: b_valid_interp.
+Hint Resolve valid_interpretation_all2: b_valid_interp.
+Hint Resolve valid_interpretation_append: b_valid_interp.
+Hint Extern 1 => eapply valid_interpretation_one; eauto: b_valid_interp.
+
+Ltac t_reducible_unused3 :=
+  match goal with
+  | H: reducible_values ((?X,?RC) :: ?theta) ?v ?T |- reducible_values ?theta' ?v ?T =>
+    unify theta theta'; apply reducible_unused3 with X RC
+  end.
+
+Lemma no_type_fvar_tail:
+  forall T x xs,
+    no_type_fvar T (x :: xs) ->
+    no_type_fvar T xs.
+Proof.
+  unfold no_type_fvar; repeat step; eauto.
+Qed.
+
+Lemma no_type_fvar_head:
+  forall T x xs,
+    no_type_fvar T (x :: xs) ->
+    x ∈ pfv T type_var ->
+    False.
+Proof.
+  unfold no_type_fvar; repeat step; eauto.
+Qed.
+
+Hint Immediate no_type_fvar_head: b_no_type_fvar.
+Hint Resolve no_type_fvar_tail: b_no_type_fvar.
+
+Lemma reducible_unused_push_all1:
+  forall theta' P theta T v,
+    sat P ->
+    no_type_fvar T (support theta') ->
+    valid_pre_interpretation P theta' ->
+    valid_interpretation theta ->
+    reducible_values (push_all P theta' ++ theta) v T ->
+    reducible_values theta v T.
+Proof.
+  induction theta';
+    repeat step || (poseNew (Mark 0 "once"); eapply IHtheta') || t_reducible_unused3 ||
+           apply valid_interpretation_append || apply valid_interpretation_all || unfold sat in * ||
+           unfold reducibility_candidate in * || instantiate_any;
+    eauto with b_no_type_fvar.
+Qed.
+
+Lemma reducible_unused_push_all2:
+  forall theta' P theta T v,
+    sat P ->
+    no_type_fvar T (support theta') ->
+    valid_pre_interpretation P theta' ->
+    valid_interpretation theta ->
+    reducible_values theta v T ->
+    reducible_values (push_all P theta' ++ theta) v T.
+Proof.
+  induction theta';
+    repeat step || (poseNew (Mark 0 "once"); eapply IHtheta') || apply reducible_unused2 ||
+           apply valid_interpretation_append || apply valid_interpretation_all || unfold sat in * ||
+           unfold reducibility_candidate in * || instantiate_any;
+    eauto with b_no_type_fvar.
+Qed.
+
+Lemma reducible_unused_push_all:
+  forall theta' P theta T v,
+    sat P ->
+    no_type_fvar T (support theta') ->
+    valid_pre_interpretation P theta' ->
+    valid_interpretation theta -> (
+      reducible_values (push_all P theta' ++ theta) v T <->
+      reducible_values theta v T
+    ).
+Proof.
+  intuition auto; eauto using reducible_unused_push_all1, reducible_unused_push_all2.
+Qed.
+
+Lemma reducible_unused_push_one1:
+  forall theta' (P: tree -> Prop) a theta T v,
+    no_type_fvar T (support theta') ->
+    P a ->
+    valid_pre_interpretation P theta' ->
+    valid_interpretation theta ->
+    reducible_values (push_one a theta' ++ theta) v T ->
+    reducible_values theta v T.
+Proof.
+  induction theta';
+    repeat step || (poseNew (Mark 0 "once"); eapply IHtheta') || t_reducible_unused3 ||
+           apply valid_interpretation_append || eapply valid_interpretation_one || unfold sat in * ||
+           unfold reducibility_candidate in * || instantiate_any;
+    eauto with b_no_type_fvar.
+Qed.
+
+Lemma reducible_unused_push_one2:
+  forall theta' (P: tree -> Prop) theta T v a,
+    P a ->
+    no_type_fvar T (support theta') ->
+    valid_pre_interpretation P theta' ->
+    valid_interpretation theta ->
+    reducible_values theta v T ->
+    reducible_values (push_one a theta' ++ theta) v T.
+Proof.
+  induction theta';
+    repeat step || apply reducible_unused2 || apply valid_interpretation_append ||
+           (eapply valid_interpretation_one; eauto);
+    eauto with b_no_type_fvar;
+    try solve [ eapply IHtheta'; eauto with b_no_type_fvar ].
+Qed.
+
+Lemma reducible_unused_push_one:
+  forall theta' (P: tree -> Prop) theta T a v,
+    P a ->
+    no_type_fvar T (support theta') ->
+    valid_pre_interpretation P theta' ->
+    valid_interpretation theta -> (
+      reducible_values (push_one a theta' ++ theta) v T <->
+      reducible_values theta v T
+    ).
+Proof.
+  intuition auto; eauto using reducible_unused_push_one1, reducible_unused_push_one2.
+Qed.
+
+Lemma valid_pre_interpretation_same:
+  forall P1 P2 theta,
+    valid_pre_interpretation P1 theta ->
+    (forall a, P1 a <-> P2 a) ->
+    valid_pre_interpretation P2 theta.
+Proof.
+  induction theta; steps; eauto with bapply_any.
+Qed.
+
+Ltac t_valid_pre_interpration_same :=
+  match goal with
+  | H: valid_pre_interpretation ?P1 ?theta |- valid_pre_interpretation ?P2 ?theta =>
+     apply valid_pre_interpretation_same with P1
+  end.
+
+Ltac t_instantiate_reducible2 :=
+  match goal with
+  | H0: no_type_fvar ?T (support ?theta'),
+    H1:reducible_values _ ?v ?T,
+    H2:is_erased_term ?v,
+    H3: forall a, _ -> reducible_values (push_one _ ?theta' ++ ?theta) a ?T -> _
+    |- _ => poseNew (Mark (v, H3) "t_instantiate_reducible2");
+          unshelve epose proof (H3 v H2 _)
+  end.
+
+Ltac t_rewrite_push_one :=
+  match goal with
+  | H1: reducible_values ?theta ?a ?A,
+    H2: reducible_values (push_one ?a ?theta' ++ ?theta) ?v ?T |- _ =>
+      rewrite (reducible_unused_push_one _ (fun a => reducible_values theta a A)) in H2 by (
+        (repeat step || apply no_type_fvar_open || t_valid_pre_interpration_same);
+        try solve [ apply_any; assumption ]
+      )
+  | H1: reducible_values ?theta ?a ?A |-
+        reducible_values (push_one ?a ?theta' ++ ?theta) ?v ?T =>
+      rewrite (reducible_unused_push_one _ (fun a => reducible_values theta a A)) by (
+        (repeat step || apply no_type_fvar_open || t_valid_pre_interpration_same);
+        try solve [ apply_any; assumption ]
+      )
+  end.
+
+Lemma strictly_positive_open_aux:
+  forall n T vars rep k,
+    size T < n ->
+    is_erased_type T ->
+    is_erased_term rep ->
+    strictly_positive T vars ->
+    strictly_positive (open k T rep) vars.
+Proof.
+  induction n; destruct T; repeat step || simp_spos || apply no_type_fvar_open || apply IHn ;
+    try omega;
+    try solve [ left; repeat step || apply no_type_fvar_open ];
+    try solve [ right; eexists; eauto; repeat step || apply no_type_fvar_open ].
+
+  right. exists X; repeat step || t_fv_open || t_listutils || rewrite is_erased_term_tfv in * by steps.
+  rewrite <- open_topen;
+    repeat step || apply IHn || autorewrite with bsize in * || apply is_erased_type_topen;
+    eauto with btwf bwf omega.
+Qed.
+
+Lemma strictly_positive_open:
+  forall T vars rep k,
+    is_erased_type T ->
+    is_erased_term rep ->
+    strictly_positive T vars ->
+    strictly_positive (open k T rep) vars.
+Proof.
+  eauto using strictly_positive_open_aux.
+Qed.
+
+Lemma push_all_cons:
+  forall X (RC: tree -> Prop) theta (P: tree -> Prop),
+    (X, fun v => forall a, P a -> RC v) :: push_all P theta = push_all P ((X, fun a => RC) :: theta).
+Proof.
+  steps.
+Qed.
+
+Lemma push_is_candidate:
+  forall (theta : interpretation) (A a : tree) (RC : tree -> Prop),
+    reducibility_candidate RC ->
+    reducible_values theta a A ->
+    reducibility_candidate (fun v : tree => reducible_values theta a A -> RC v).
+Proof.
+  repeat step || unfold non_empty in * || unfold reducibility_candidate in * || instantiate_any;
+    eauto with bfv bwf.
+Qed.
+
+Lemma push_all_is_candidate:
+  forall (theta : interpretation) (A : tree) (RC : tree -> Prop),
+    reducibility_candidate RC ->
+    non_empty theta A ->
+    reducibility_candidate (fun v : tree => forall a, reducible_values theta a A -> RC v).
+Proof.
+  repeat step || unfold non_empty in * || unfold reducibility_candidate in * || instantiate_any;
+    eauto with bfv bwf.
+Qed.
+
+Ltac find_exists2 :=
+  match goal with
+  | H1: reducible_values ?theta ?a ?T1,
+    H2: reducible_values ?theta ?v (open 0 ?T2 ?a)
+    |- _ =>
+    exists a
+  end.
+
+Lemma no_type_fvar_strictly_positive:
+  forall T vars,
+    is_erased_type T ->
+    no_type_fvar T vars ->
+    strictly_positive T vars.
+Proof.
+  induction T; repeat step || simp_spos || destruct_tag || unfold no_type_fvar in * || apply_any || left;
+    try solve [ eapply_any; eauto; repeat step || t_listutils ].
+Qed.
+
+Ltac t_red_is_val :=
+  eapply red_is_val; eauto;
+    repeat step || apply valid_interpretation_append || eapply valid_interpretation_one ||
+    eauto with b_valid_interp; steps;
+    eauto with bapply_any.
+
+Hint Extern 50 => solve [ t_red_is_val ]: b_red_is_val.
+
+Lemma sat_p:
+  forall P theta a A,
+    reducible_values theta a A ->
+    (forall a, P a <-> reducible_values theta a A) ->
+    sat P.
+Proof.
+  unfold sat; steps; eauto with bapply_any.
+Qed.
+
+Lemma no_type_fvar_in_topen:
+  forall T vars k X,
+    no_type_fvar T vars ->
+    ~(X ∈ vars) ->
+    no_type_fvar (topen k T (fvar X type_var)) vars.
+Proof.
+  unfold no_type_fvar; repeat step || t_fv_open || t_listutils; eauto.
+Qed.
+
+Definition similar_sets (rel: M nat nat) (vars vars': list nat): Prop :=
+  forall x y,
+    lookup Nat.eq_dec rel x = Some y ->
+    lookup Nat.eq_dec (swap rel) y = Some x ->
+    (x ∈ vars <-> y ∈ vars').
+
+Opaque strictly_positive.
+
+Lemma equal_with_relation_pfv:
+  forall T T' rel X,
+    equal_with_relation rel T T' ->
+    X ∈ pfv T type_var ->
+    exists X',
+      X' ∈ pfv T' type_var /\
+      lookup Nat.eq_dec rel X = Some X' /\
+      lookup Nat.eq_dec (swap rel) X' = Some X.
+Proof.
+  induction T;
+    repeat match goal with
+           | H1: equal_with_relation ?rel ?T ?T',
+             H2: ?X ∈ pfv ?T type_var,
+             H3: forall _ _ _, _ -> _ -> _ |- _ => pose proof (H3 _ _ _ H1 H2); clear H3
+           | _ => step || t_listutils || destruct_tag
+           end; eauto;
+      try solve [ eexists; repeat step || t_listutils; eauto ].
+Qed.
+
+Ltac t_equal_with_relation_pfv :=
+  match goal with
+  | H1: equal_with_relation ?rel ?T ?T',
+    H2: ?X ∈ pfv ?T type_var |- _ =>
+    poseNew (Mark H1 "equal_with_relation_pfv");
+    pose proof (equal_with_relation_pfv _ _ _ _ H1 H2)
+  end.
+
+Lemma equal_with_relation_pfv2:
+  forall T T' rel X',
+    equal_with_relation rel T T' ->
+    X' ∈ pfv T' type_var ->
+    exists X,
+      X ∈ pfv T type_var /\
+      lookup Nat.eq_dec rel X = Some X' /\
+      lookup Nat.eq_dec (swap rel) X' = Some X.
+Proof.
+  intros.
+  apply equal_with_relation_swap in H.
+  repeat step || t_equal_with_relation_pfv || eexists || rewrite swap_twice in *; eauto.
+Qed.
+
+Ltac t_equal_with_relation_pfv2 :=
+  match goal with
+  | H1: equal_with_relation ?rel ?T ?T',
+    H2: ?X ∈ pfv ?T' type_var |- _ =>
+    poseNew (Mark H1 "equal_with_relation_pfv2");
+    pose proof (equal_with_relation_pfv2 _ _ _ _ H1 H2)
+  | _ => t_equal_with_relation_pfv
+  end.
+
+Lemma no_type_fvar_rename:
+  forall T T' vars vars' rel,
+    no_type_fvar T vars ->
+    equal_with_relation rel T T' ->
+    similar_sets rel vars vars' ->
+    no_type_fvar T' vars'.
+Proof.
+  unfold no_type_fvar, similar_sets;
+    repeat step || t_equal_with_relation_pfv2 || t_lookup_same;
+    eauto with beapply_any.
+Qed.
+
+Lemma strictly_positive_rename_aux:
+  forall n T T' vars vars' rel,
+    size T < n ->
+    strictly_positive T vars ->
+    equal_with_relation rel T T' ->
+    similar_sets rel vars vars' ->
+    strictly_positive T' vars'.
+Proof.
+  induction n; destruct T;
+    repeat (intuition auto) || cbn -[equal_with_relation] in * || simp_spos || destruct_tag; try omega;
+    match goal with
+    | H: equal_with_relation  _ _ ?T |- _ => is_var T; destruct T; simpl in H
+    end;
+    repeat match goal with
+           | H1: equal_with_relation ?rel ?T ?T',
+             H2: strictly_positive ?T ?vars |-
+               strictly_positive ?T' ?vars' =>
+             apply IHn with T vars rel
+           | _ => step || destruct_tag || simp_spos
+           end;
+    try omega;
+    eauto using no_type_fvar_rename.
+
+  right.
+  exists (makeFresh ((X :: nil) :: pfv T'3 type_var :: nil));
+    repeat step; try finisher.
+
+  match goal with
+  | H1: equal_with_relation ?rel _ _,
+    H2: strictly_positive ?T (?X :: nil) |-
+      strictly_positive (topen 0 ?T' (fvar ?M type_var)) ?vars' =>
+    apply IHn with T (X :: nil) ((X,M) :: rel)
+  end;
+    repeat unfold similar_sets || step || autorewrite with bsize in * || apply equal_with_relation_topen;
+      try omega;
+      try finisher.
+Qed.
+
+Lemma strictly_positive_rename:
+  forall T T' vars vars' rel,
+    strictly_positive T vars ->
+    equal_with_relation rel T T' ->
+    similar_sets rel vars vars' ->
+    strictly_positive T' vars'.
+Proof.
+  eauto using strictly_positive_rename_aux.
+Qed.
+
+Lemma topen_swap:
+  forall T i j rep,
+    twf rep 0 ->
+    topen i (swap_type_holes T j i) rep =
+    swap_type_holes (topen j T rep) j i.
+Proof.
+  induction T; repeat step || tequality || rewrite (swap_nothing _ 0);
+    try omega.
+Qed.
+
+Lemma pfv_swap:
+  forall T i j tag, pfv (swap_type_holes T i j) tag = pfv T tag.
+Proof.
+  induction T; steps.
+Qed.
+
+Lemma no_type_fvar_swap:
+  forall T vars i j,
+    no_type_fvar T vars ->
+    no_type_fvar (swap_type_holes T i j) vars.
+Proof.
+  unfold no_type_fvar; repeat step || rewrite pfv_swap in *; eauto.
+Qed.
+
+Lemma topen_swap2:
+  forall T k i j rep,
+    twf rep 0 ->
+    k <> i ->
+    k <> j ->
+    topen k (swap_type_holes T j i) rep =
+    swap_type_holes (topen k T rep) j i.
+Proof.
+  induction T; repeat step || tequality || rewrite (swap_nothing _ 0);
+    try omega.
+Qed.
+
+Lemma strictly_positive_swap_aux:
+  forall n T vars i j,
+    size T < n ->
+    strictly_positive T vars ->
+    strictly_positive (swap_type_holes T i j) vars.
+Proof.
+  induction n; destruct T; repeat step || simp_spos || apply_any;
+    try omega;
+    eauto using no_type_fvar_swap.
+  right; exists X; repeat step || rewrite pfv_swap in *.
+  rewrite topen_swap2; steps.
+  apply IHn; repeat step || autorewrite with bsize in *; try omega.
+Qed.
+
+Lemma strictly_positive_swap:
+  forall T vars i j,
+    strictly_positive T vars ->
+    strictly_positive (swap_type_holes T i j) vars.
+Proof.
+  eauto using strictly_positive_swap_aux.
+Qed.
+
+Lemma strictly_positive_topen_aux:
+  forall n T vars k X,
+    size T < n ->
+    strictly_positive T vars ->
+    ~(X ∈ vars) ->
+    strictly_positive (topen k T (fvar X type_var)) vars.
+Proof.
+  induction n; destruct T; repeat step || simp_spos || apply IHn;
+    eauto using no_type_fvar_in_topen;
+    try omega.
+  right; exists (makeFresh ((X0 :: nil) :: (X :: nil) :: pfv T3 type_var :: pfv (topen (S k) T3 (fvar X type_var)) type_var :: nil)); steps; try finisher.
+
+  rewrite open_swap; repeat step.
+  apply IHn; repeat step || autorewrite with bsize in *;
+    try omega;
+    try finisher.
+  rewrite topen_swap; steps.
+  apply strictly_positive_swap.
+  match goal with
+  | H2: strictly_positive (topen 0 ?T (fvar ?X type_var)) (?X :: nil) |-
+      strictly_positive (topen 0 ?T (fvar ?M type_var)) (?M :: nil) =>
+    apply strictly_positive_rename with (topen 0 T (fvar X type_var)) (X :: nil) ((X,M) :: idrel (pfv T type_var))
+  end;
+    unfold similar_sets;
+    repeat step || apply equal_with_relation_topen;
+    try finisher;
+    eauto using equal_with_relation_refl2;
+    eauto using equal_with_idrel.
+Qed.
+
+Lemma equivalent_with_relation_permute2:
+  forall theta1 theta2 (RC : tree -> Prop) X Y l,
+    ~(X ∈ support theta1) ->
+    equivalent_with_relation
+      ((Y, X) :: idrel l)
+        ((Y, RC) :: theta1 ++ theta2)
+        (theta1 ++ (X, RC) :: theta2).
+Proof.
+  unfold equivalent_with_relation, equivalent_rc_at;
+    repeat match goal with
+           | |- exists r, Some ?R = Some r /\ _ => exists R
+           | |- exists r, _ /\ equivalent_rc r ?R => exists R
+           | H: _ |- _ => rewrite lookup_remove2 in H by steps
+           | _ => rewrite lookup_remove2 by steps
+           | _ => step || t_lookup_rewrite || t_idrel || t_lookup || t_listutils ||
+                 rewrite obvious_lookup in * by steps ||
+                 t_lookupor || t_lookup_same
+           end;
+    eauto using equivalent_rc_refl.
+Qed.
+
+Lemma reducible_rename_permute:
+  forall T theta1 theta2 X Y (RC : tree -> Prop) v,
+    valid_interpretation theta1 ->
+    valid_interpretation theta2 ->
+    reducibility_candidate RC ->
+    ~(Y ∈ support theta1) ->
+    ~(X ∈ pfv T type_var) ->
+    ~(Y ∈ pfv T type_var) ->
+    reducible_values ((X, RC) :: theta1 ++ theta2) v (topen 0 T (fvar X type_var)) ->
+    reducible_values (theta1 ++ (Y, RC) :: theta2) v (topen 0 T (fvar Y type_var)).
+Proof.
+  intros.
+  eapply (reducible_rename _ _ _ _ _ ((X,Y) :: idrel (pfv T type_var))); eauto;
+    repeat step || apply valid_interpretation_append || apply equal_with_relation_topen;
+    eauto using equal_with_idrel.
+
+  apply equivalent_with_relation_permute2; steps.
+Qed.
+
+Lemma support_push_one:
+  forall theta a,
+    support (push_one a theta) = support theta.
+Proof.
+  unfold push_one; repeat step || rewrite support_mapValues.
+Qed.
+
+Lemma support_push_all:
+  forall theta P,
+    support (push_all P theta) = support theta.
+Proof.
+  unfold push_one; repeat step || rewrite support_mapValues.
 Qed.
 
 Lemma strictly_positive_topen:
-  forall T i j R,
-    is_erased_type T ->
-    is_erased_type R ->
-    twf R 0 ->
-    strictly_positive T i ->
-    strictly_positive (topen j T R) i.
+  forall T vars k X,
+    strictly_positive T vars ->
+    ~(X ∈ vars) ->
+    strictly_positive (topen k T (fvar X type_var)) vars.
 Proof.
-  induction T; steps;
-    eauto using twf_positive2;
-    eauto using no_type_lvar_in_topen.
+  eauto using strictly_positive_topen_aux.
 Qed.
 
-Lemma no_type_var_positive:
-  forall T k,
-    is_erased_type T ->
-    no_type_lvar T k ->
-    strictly_positive T k.
+Lemma swap_idrel:
+  forall l, swap (idrel l) = idrel l.
 Proof.
-  induction T; steps; try omega.
+  induction l; steps.
 Qed.
 
-Lemma no_type_lvar_topen:
-  forall T k R,
-    no_type_lvar T k ->
-    is_erased_type T ->
-    topen k T R = T.
+Lemma idrel_lookup2:
+  forall x y l eq_dec, lookup eq_dec (idrel l) x = Some y -> x = y /\ x ∈ l.
 Proof.
-  induction T; repeat step || tequality || t_topen_none.
+  induction l; repeat step || eapply_any || instantiate_any.
 Qed.
 
-Lemma strictly_positive_push_forall:
-  forall measure T theta A B v,
-    (size T, index T) = measure ->
-    strictly_positive T 0 ->
-    wf T 0 ->
-    twf T 1 ->
-    wf A 0 ->
-    twf A 0 ->
-    wf B 1 ->
-    twf B 0 ->
-    valid_interpretation theta ->
-    non_empty theta A ->
-    is_erased_type A ->
-    is_erased_type B ->
-    is_erased_type T ->
-    (forall a,
-      reducible_values theta a A ->
-      reducible_values theta v (topen 0 T (open 0 B a))) ->
-    reducible_values theta v (topen 0 T (T_forall A B)).
-Proof.
-  induction measure as [ PP HH ] using measure_induction; intros; t_instantiate_non_empty; destruct T;
-    repeat match goal with
-    | _ =>
-      step ||
-      simp_red ||
-      t_topen_none ||
-      t_instantiate_reducible ||
-      find_reducible_value ||
-      reducibility_choice ||
-      t_deterministic_star ||
-      (* t_reduces_to || *)
-      ( progress unfold reduces_to in * ) ||
-      find_smallstep_value ||
-      apply strictly_positive_open ||
-      apply left_lex ||
-      apply_induction HH ||
-      find_exists ||
-      ( progress autorewrite with bsize in * ) ||
-      (rewrite open_topen in * by (steps; eauto with btwf; eauto with bwf)) ||
-      (rewrite no_type_lvar_topen in * by (repeat step || apply no_type_lvar_open || apply is_erased_type_open; eauto with btwf))
-    end;
-    try omega;
-    eauto using reducible_values_closed;
-    eauto with berased bwf btwf;
-    eauto using no_type_var_positive;
-    try solve [ apply twf_open; eauto with btwf ];
-    t_closer.
+Ltac t_idrel_lookup2 :=
+  match goal with
+  | H: lookup _ (idrel ?l) ?x = Some ?y |- _ => pose proof (idrel_lookup2 _ _ _ _ H); clear H
+  end.
 
-  (** Polymorphic type **)
-  - exists (makeFresh (
-           support theta ::
-           pfv A type_var ::
-           pfv T type_var ::
-           pfv B type_var ::
-           pfv (topen 1 T (T_forall A B)) type_var :: nil));
-      repeat step || finisher || t_instantiate_rc || find_smallstep_value;
-        try solve [ repeat unfold closed_term, closed_value in * || step ].
-
-    rewrite open_swap; steps; eauto with omega.
-    apply_induction HH;
-      repeat
-        step ||
-        apply left_lex ||
-        (progress autorewrite with bsize in * ) ||
-        apply strictly_positive_swap ||
-        apply twf_topen ||
-        apply is_erased_type_topen ||
-        apply non_empty_extend ||
-        t_deterministic_star ||
-        apply wf_topen;
-      try finisher;
-      eauto with bwf btwf omega berased;
-      eauto 2 using red_is_val with step_tactic.
-
-    apply reducible_unused3 in H27; steps; try finisher.
-
-    rewrite open_swap;
-      repeat step || rewrite swap_holes_twice ||
-             t_instantiate_reducible || t_instantiate_rc ||
-             unfold reduces_to in * || t_deterministic_star ||
-             simp_red || t_reducible_rename_one || t_fv_open ||
-             t_listutils ||
-             unshelve eauto using valid_interpretation_cons with btwf btwf2 ||
-             unshelve eauto using valid_interpretation_cons, red_is_val;
-      try finisher;
-      eauto using fv_in_reducible_val.
-
-  (** Recursive type at 0 **)
-  - left.
-      repeat step || simp_red ||
-             t_instantiate_reducible || apply_induction HH || apply left_lex ||
-             t_deterministic_star ||
-             t_topen_none; eauto with omega.
-
-  (** Recursive type at n+1 **)
-  - right.
-      exists n'0, v'0, (makeFresh (
-                       support theta ::
-                       pfv A type_var ::
-                       pfv n'0 type_var ::
-                       pfv (topen 0 T2 (T_forall A B)) type_var ::
-                       pfv (topen 1 T3 (T_forall A B)) type_var ::
-                       nil));
-      repeat step || simp_red ||
-             t_instantiate_reducible || apply_induction HH || apply left_lex ||
-             t_deterministic_star ||
-             t_topen_none;
-        eauto with omega;
-        try finisher.
-
-      remember (makeFresh (
-                       support theta ::
-                       pfv A type_var ::
-                       pfv n'0 type_var ::
-                       pfv (topen 0 T2 (T_forall A B)) type_var ::
-                       pfv (topen 1 T3 (T_forall A B)) type_var ::
-                       nil)) as M.
-
-      apply reducibility_subst_head2;
-        repeat
-          step || t_listutils ||
-          apply is_erased_topen ||
-          apply is_erased_type_topen ||
-          apply twf_topen ||
-          apply wf_topen;
-        try finisher;
-        eauto with btwf;
-        eauto with bwf.
-
-Set Nested Proofs Allowed.
-Lemma topen_rec:
-  forall k n T0 Ts R,
-    twf n 0 ->
-    topen k (T_rec n T0 Ts) R = T_rec n (topen k T0 R) (topen (S k) Ts R).
-Proof.
-  repeat step || tequality || rewrite topen_none; eauto with btwf omega.
-Qed.
-
-      rewrite open_swap;
-        repeat step || apply twf_topen;
-        eauto with omega;
-        eauto with btwf.
-
-      rewrite <- topen_rec; eauto with btwf.
-      define M2 (makeFresh (
-                     pfv (swap_type_holes T3 0 1) type_var ::
-                     pfv (T_rec n'0 T2 T3) type_var ::
-                     nil
-                )).
-      rewrite (topen_twice _ _ _ M2); steps; eauto with btwf; try finisher.
-
-    apply_induction HH;
-      repeat
-        step ||
-        apply left_lex ||
-        (progress autorewrite with bsize in * ) ||
-        apply strictly_positive_swap ||
-        apply twf_topen ||
-        apply is_erased_type_topen ||
-        apply non_empty_extend ||
-        t_deterministic_star ||
-        apply wf_topen;
-      try finisher;
-      eauto with bwf btwf omega berased;
-      eauto 2 using red_is_val with step_tactic;
-      eauto using reducibility_is_candidate.
-
-    + admit. (* use multiset measure *)
-    +
-
-Lemma strictly_positive_close:
-  forall T k1 k2 rep,
-    twf rep 0 ->
-    strictly_positive T k1 ->
-    strictly_positive (open k2 T rep) k1.
-Proof.
-  induction T; steps; eauto using twf_open with btwf omega.
-Qed.
-
-      remember (makeFresh (
-                       support theta ::
-                       pfv A type_var ::
-                       pfv n'0 type_var ::
-                       pfv (topen 0 T2 (T_forall A B)) type_var ::
-                       pfv (topen 1 T3 (T_forall A B)) type_var ::
-                       nil)) as M.
-      
-
-     (*
-    topen 0 (topen 1 A R) (topen 0 B R)
-*)
-(*
-*)
-    (*
-    assert (
-      topen 0 (topen 1 A (topen 0 B R)) R
-      topen 0 (t_close 0 (topen 1 A (topen 0 B X)) X) R
+Lemma reducible_unused_middle:
+  forall X RC theta1 theta2 v T,
+    valid_interpretation theta1 ->
+    valid_interpretation theta2 ->
+    reducibility_candidate RC ->
+    no_type_fvar T (support theta1) -> (
+      reducible_values ((X,RC) :: theta1 ++ theta2) v T <->
+      reducible_values ((X,RC) :: theta2) v T
     ).
-*)
-Admitted.
-
-Lemma strictly_positive_pull_forall:
-  forall T theta A B v a,
-    strictly_positive T 0 ->
-    wf T 0 ->
-    twf T 1 ->
-    wf A 0 ->
-    twf A 0 ->
-    wf B 1 ->
-    twf B 0 ->
-    valid_interpretation theta ->
-    reducible_values theta a A ->
-    reducible_values theta v (topen 0 T (T_forall A B)) ->
-    reducible_values theta v (topen 0 T (open 0 B a)).
 Proof.
-(*  induction T;
-    repeat t_topen_none || step ||
-      simp reducible_values in * ||
-      (rewrite topen_none in * by t_rewrite);
-    eauto 6 with berased; eauto 11. *)
-Admitted.
+  repeat step.
+  - apply reducible_rename with T ((X, RC) :: theta1 ++ theta2) (idrel (pfv T type_var));
+      repeat step || apply valid_interpretation_append || (rewrite swap_idrel in * by steps) ||
+             t_idrel_lookup2 || t_lookupor || t_lookup_rewrite || t_lookup ||
+             unfold equivalent_with_relation, equivalent_rc_at || unfold no_type_fvar in * ||
+             unshelve eauto with falsity || exact True;
+      eauto using equal_with_idrel;
+      eauto using equivalent_rc_refl;
+    unfold equivalent_with_relation.
+
+    exists rc2; repeat step || rewrite lookupRight || apply lookupNoneSupport; eauto using equivalent_rc_refl.
+  - apply reducible_rename with T ((X, RC) :: theta2) (idrel (pfv T type_var));
+      repeat step || apply valid_interpretation_append || (rewrite swap_idrel in * by steps) ||
+             t_idrel_lookup2 || t_lookupor || t_lookup_rewrite || t_lookup ||
+             unfold equivalent_with_relation, equivalent_rc_at || unfold no_type_fvar in * ||
+             unshelve eauto with falsity || exact True;
+      eauto using equal_with_idrel;
+      eauto using equivalent_rc_refl;
+    unfold equivalent_with_relation.
+
+    exists rc1; repeat step || rewrite lookupRight || apply lookupNoneSupport; eauto using equivalent_rc_refl.
+Qed.
