StrictPositivityPush.v
@@ -1,0 +1,300 @@
+Require Import Equations.Equations.
+Require Import Equations.Subterm.
+
+Require Import Omega.
+
+Require Import Coq.Strings.String.
+Require Import Coq.Lists.List.
+
+Require Import Termination.StarInversions.
+Require Import Termination.StarRelation.
+Require Import Termination.SmallStep.
+Require Import Termination.Syntax.
+Require Import Termination.Trees.
+Require Import Termination.Tactics.
+Require Import Termination.Equivalence.
+Require Import Termination.OpenTOpen.
+
+Require Import Termination.SizeLemmas.
+
+Require Import Termination.WFLemmas.
+Require Import Termination.TWFLemmas.
+Require Import Termination.ErasedTermLemmas.
+
+Require Import Termination.ReducibilityCandidate.
+Require Import Termination.ReducibilityDefinition.
+Require Import Termination.ReducibilityLemmas.
+Require Import Termination.RedTactics.
+Require Import Termination.ReducibilityMeasure.
+Require Import Termination.ReducibilitySubst.
+Require Import Termination.ReducibilityRenaming.
+Require Import Termination.ReducibilityUnused.
+Require Import Termination.RedTactics2.
+
+Require Import Termination.IdRelation.
+Require Import Termination.EqualWithRelation.
+
+Require Import Termination.EquivalentWithRelation.
+Require Import Termination.AssocList.
+Require Import Termination.Sets.
+Require Import Termination.Freshness.
+Require Import Termination.SwapHoles.
+Require Import Termination.ListUtils.
+Require Import Termination.TOpenTClose.
+Require Import Termination.StrictPositivity.
+
+Require Import Termination.FVLemmas.
+
+Opaque makeFresh.
+Opaque Nat.eq_dec.
+Opaque reducible_values.
+Opaque strictly_positive.
+
+Lemma strictly_positive_push_forall_fvar:
+  forall (n : nat) (theta : interpretation) (theta' : list (nat * (tree -> tree -> Prop))) X (A : tree) v P,
+    non_empty theta A ->
+    (forall a : tree,
+        reducible_values theta a A ->
+        reducible_values (push_one a theta' ++ theta) v (fvar X type_var)) ->
+    (forall a, P a <-> reducible_values theta a A) ->
+    reducible_values (push_all P theta' ++ theta) v (fvar X type_var).
+Proof.
+  unfold push_all, push_one;
+  intros; t_instantiate_non_empty;
+    repeat match goal with
+           | H1: forall a, ?P a <-> reducible_values ?theta a ?A, H2: ?P ?a |- _ =>
+              poseNew (Mark H2 "equiv_inst");
+              pose proof (proj1 (H1 a) H2)
+           | _ =>
+             t_lookup_same || step || simp_red || t_lookupor || t_lookup_rewrite || t_lookupMap2 || t_instantiate_reducible || t_lookup || rewrite support_mapValues in * || t_listutils
+           end.
+Qed.
+
+Hint Resolve strictly_positive_push_forall_fvar: b_push.
+
+Ltac apply_induction H :=
+  match goal with
+  | H1: non_empty ?theta ?A |- reducible_values (push_all _ _ ++ _) _ ?T =>
+      apply H with (size T, index T) A
+  end.
+
+Lemma strictly_positive_push_forall:
+  forall measure T theta theta' A v P,
+    (size T, index T) = measure ->
+    wf T 0 ->
+    twf T 0 ->
+    wf A 0 ->
+    twf A 0 ->
+    valid_interpretation theta ->
+    non_empty theta A ->
+    valid_pre_interpretation P theta' ->
+    strictly_positive T (support theta') ->
+    is_erased_type A ->
+    is_erased_type T ->
+    (forall a,
+      reducible_values theta a A ->
+      reducible_values (push_one a theta' ++ theta) v T) ->
+    (forall a, P a <-> reducible_values theta a A) ->
+    reducible_values (push_all P theta' ++ theta) v T.
+Proof.
+  induction measure as [ PP HH ] using measure_induction; intros; t_instantiate_non_empty;
+    destruct T; try destruct_tag;
+    eauto with b_push;
+    repeat match goal with
+    | |- closed_term _ => solve [ t_closing; eauto with bfv bwf b_valid_interp ]
+    | |- wf _ _ => solve [ t_closing; repeat step || apply wf_open ]
+    | _ =>
+      step ||
+      simp_red ||
+      simp_spos ||
+      t_topen_none ||
+      t_instantiate_reducible ||
+      t_instantiate_reducible2 ||
+      find_reducible_value ||
+      reducibility_choice ||
+      t_deterministic_star ||
+      t_rewrite_push_one ||
+      ( progress unfold reduces_to in * ) ||
+      find_smallstep_value ||
+      apply strictly_positive_open ||
+      apply left_lex ||
+      find_exists ||
+      find_exists2 ||
+      ( progress autorewrite with bsize in * ) ||
+      (rewrite reducible_unused_push_all in * by (steps; eauto using sat_p)) ||
+      (rewrite reducible_unused_push_one in * by (eauto; steps)) ||
+      (rewrite open_topen in * by (steps; eauto with btwf; eauto with bwf)) ||
+      (rewrite no_type_lvar_topen in * by (repeat step || apply no_type_lvar_open || apply is_erased_type_open; eauto with btwf)) ||
+      apply_induction HH
+    end;
+    try omega;
+    eauto using reducible_values_closed;
+    eauto with berased bwf btwf;
+    try solve [ apply twf_open; eauto with btwf ];
+    eauto with b_red_is_val;
+    eauto using no_type_fvar_strictly_positive;
+    try solve [ apply_any; assumption ].
+
+  (** Polymorphic type **)
+  - exists (makeFresh (
+           support theta ::
+           pfv A type_var ::
+           pfv T type_var ::
+           support (push_all (fun a : tree => reducible_values theta a A) theta' ++ theta) ::
+           support (push_all (fun a : tree => reducible_values theta a A) theta') ::
+           support (push_all P theta' ++ theta) ::
+           support (push_all P theta') ::
+           support (push_one a theta') ::
+           support theta' ::
+           nil));
+      repeat step || finisher || t_instantiate_rc || find_smallstep_value;
+        try solve [ repeat unfold closed_term, closed_value in * || step ].
+
+    lazymatch goal with
+    | |- reducible_values ((?X,?RC) :: ?g1 ++ ?g2) _ (topen 0 ?T ?rep) =>
+      apply reducible_rename with (topen 0 T rep) (g1 ++ (X,RC) :: g2)
+                                  (idrel (X :: support g1 ++ support g2 ++ pfv T type_var))
+    end;
+      repeat step || apply valid_interpretation_append ||
+             apply push_all_is_candidate || apply equivalent_with_relation_permute ||
+             apply equal_with_relation_refl2 ||
+             rewrite idrel_lookup || t_fv_open ||
+             rewrite idrel_lookup_swap || t_fv_open ||
+             t_listutils;
+        eauto with b_valid_interp;
+        eauto using reducibility_is_candidate;
+        try solve [ unfold equivalent_rc; steps; eauto ];
+        try solve [ apply valid_interpretation_all; eauto using sat_p ];
+        try finisher.
+
+    apply_induction HH;
+      repeat
+        step ||
+        apply left_lex ||
+        (progress autorewrite with bsize in * ) ||
+        apply strictly_positive_swap ||
+        apply twf_topen ||
+        apply is_erased_type_topen ||
+        apply non_empty_extend ||
+        t_deterministic_star ||
+        apply strictly_positive_topen ||
+        apply wf_topen;
+      try finisher;
+      eauto with bwf btwf omega berased;
+      eauto 2 using red_is_val with step_tactic;
+      eauto with b_red_is_val;
+      try solve [ apply_any; assumption ].
+
+    + apply reducible_unused3 in H14; repeat step || t_instantiate_reducible || simp_red || t_instantiate_rc ||
+                                             t_deterministic_star ||
+                                             unfold reduces_to in *; try finisher;
+        eauto with b_red_is_val.
+      apply reducible_rename_permute with X1;
+        repeat step || eapply valid_interpretation_one || eauto || rewrite support_push_one in *; eauto with bapply_any;
+          try finisher.
+
+   + apply reducible_unused2; steps; try finisher; eauto with bapply_any.
+   + apply reducible_unused3 in H14; repeat step; try finisher; eauto with bapply_any.
+
+  (** Recursive type at 0: case where the recursive type is itself strictly positive **)
+  - left.
+      repeat step || simp_red ||
+             t_instantiate_reducible || apply_induction HH || apply left_lex ||
+             t_deterministic_star ||
+             t_topen_none; eauto with omega;
+        eauto with bapply_any.
+
+  (** Recursive type at n+1: case where the variables do not appear in the recursive type **)
+  - right.
+      exists n'0, v'0, (makeFresh (
+                       support theta ::
+                       support theta' ::
+                       pfv A type_var ::
+                       pfv T2 type_var ::
+                       pfv T3 type_var ::
+                       pfv n'0 type_var ::
+                       support (push_all P theta' ++ theta) ::
+                       nil));
+      repeat step || simp_red ||
+             t_instantiate_reducible ||
+             t_deterministic_star ||
+             t_topen_none;
+        eauto with omega;
+        try finisher.
+
+      repeat
+        rewrite reducible_unused_middle in * by (
+          repeat step || t_listutils ||
+                 apply valid_interpretation_append ||
+                 apply valid_interpretation_all ||
+                 (eapply valid_interpretation_one; eauto) ||
+                 apply no_type_fvar_in_topen ||
+                 rewrite support_push_one in * ||
+                 rewrite support_push_all in * ||
+                 apply reducibility_is_candidate;
+          eauto using sat_p;
+          try solve [ apply_any; assumption ];
+          try finisher
+        ).
+
+Hint Resolve valid_interpretation_append: b_valid_interp.
+Hint Extern 1 => eapply valid_interpretation_one; eauto: b_valid_interp.
+
+Ltac success t := (t; fail) || (t; []).
+
+Ltac t_rewrite_unused_push_one :=
+  rewrite reducible_unused_push_one in *; (
+    repeat step || t_listutils || unfold no_type_fvar in * ||
+           (rewrite is_erased_term_tfv in * by (steps; eauto with berased)) ||
+           rewrite support_push_all in * || rewrite support_push_one in *;
+    eauto using sat_p; eauto with bapply_any; try finisher
+  ).
+
+Ltac t_rewrite_unused_push_all :=
+  rewrite reducible_unused_push_all in *; (
+    repeat step || t_listutils || unfold no_type_fvar in * ||
+           (rewrite is_erased_term_tfv in * by (steps; eauto with berased)) ||
+           rewrite support_push_all in * || rewrite support_push_one in *;
+    eauto using sat_p; eauto with bapply_any; try finisher
+  ).
+
+      eapply reducible_rename_one_rc; eauto;
+        repeat step ||
+               (success t_rewrite_unused_push_all) ||
+               (success t_rewrite_unused_push_one) ||
+               apply reducibility_is_candidate ||
+               unfold equivalent_rc;
+        eauto using sat_p with b_valid_interp bapply_any;
+        try finisher.
+
+  (** Recursive type at n+1: case where the recursive type is itself strictly positive **)
+  - right.
+      exists n'0, v'0, (makeFresh (
+                       support theta ::
+                       support theta' ::
+                       pfv A type_var ::
+                       pfv T2 type_var ::
+                       pfv T3 type_var ::
+                       pfv n'0 type_var ::
+                       support (push_all P theta' ++ theta) ::
+                       nil));
+      repeat step || simp_red ||
+             t_instantiate_reducible ||
+             t_deterministic_star ||
+             t_topen_none;
+        eauto with omega;
+        try finisher.
+
+      remember  (makeFresh (
+                       support theta ::
+                       support theta' ::
+                       pfv A type_var ::
+                       pfv T2 type_var ::
+                       pfv T3 type_var ::
+                       pfv n'0 type_var ::
+                       support (push_all P theta' ++ theta) ::
+                       nil)) as M.
+
+
+      erewrite push_all_cons.
+      apply HH.
